src/Inline.v
@@ -4,9 +4,14 @@ Require Import Syntax.
 
 Set Implicit Arguments.
 
+Ltac destruct_existT :=
+  repeat match goal with
+           | [H: existT _ _ _ = existT _ _ _ |- _] =>
+             (apply Eqdep.EqdepTheory.inj_pair2 in H; subst)
+         end.
+
 Section Phoas.
   Variable type: Kind -> Type.
-  Variable getDefault: forall (k: Kind), type k.
 
   Definition inlineArg {argT retT} (a: Expr type argT)
              (m: type argT -> Action type retT): Action type retT :=
@@ -31,123 +36,280 @@ Section Phoas.
       | Return e => Let_ e a2
     end.
 
-  Fixpoint inlineActionOnce {retT} (a: Action type retT)
-           (dms: list (DefMethT type)): Action type retT :=
+  Fixpoint inlineDm {retT} (a: Action type retT)
+           (dm: DefMethT type): Action type retT :=
     match a with
       | MCall name sig ar cont =>
-        match getMethod name dms with
-          | Some dm =>
-            match SignatureT_dec (objType dm) sig with
-              | left e => appendAction (inlineArg ar (eq_rect _ _ (objVal dm) _ e)) cont
-              | right _ =>
-                MCall name sig ar (fun ak => inlineActionOnce (cont ak) dms)
-            end
-          | None =>
-            MCall name sig ar (fun ak => inlineActionOnce (cont ak) dms)
-        end
-      | Let_ _ ar cont => Let_ ar (fun a => inlineActionOnce (cont a) dms)
-      | ReadReg reg k cont => ReadReg reg k (fun a => inlineActionOnce (cont a) dms)
-      | WriteReg reg _ e cont => WriteReg reg e (inlineActionOnce cont dms)
-      | IfElse ce _ ta fa cont => IfElse ce (inlineActionOnce ta dms)
-                                         (inlineActionOnce fa dms)
-                                         (fun a => inlineActionOnce (cont a) dms)
-      | Assert_ ae cont => Assert_ ae (inlineActionOnce cont dms)
+        if string_dec name (attrName dm) then
+          match SignatureT_dec (objType (attrType dm)) sig with
+            | left e => appendAction (inlineArg ar (eq_rect _ _ (objVal (attrType dm)) _ e))
+                                     (* (fun ak => inlineDm (cont ak) dm) *) cont
+            | right _ =>
+              MCall name sig ar (fun ak => inlineDm (cont ak) dm)
+          end
+        else
+          MCall name sig ar (fun ak => inlineDm (cont ak) dm)
+      | Let_ _ ar cont => Let_ ar (fun a => inlineDm (cont a) dm)
+      | ReadReg reg k cont => ReadReg reg k (fun a => inlineDm (cont a) dm)
+      | WriteReg reg _ e cont => WriteReg reg e (inlineDm cont dm)
+      | IfElse ce _ ta fa cont => IfElse ce (inlineDm ta dm) (inlineDm fa dm)
+                                         (fun a => inlineDm (cont a) dm)
+      | Assert_ ae cont => Assert_ ae (inlineDm cont dm)
       | Return e => Return e
     end.
 
-  Fixpoint inlineAction {retT} (a: Action type retT) (dms: list (DefMethT type))
+  Fixpoint inlineDms {retT} (a: Action type retT)
+           (dms: list (DefMethT type)): Action type retT :=
+    match dms with
+      | nil => a
+      | dm :: dms' => inlineDms (inlineDm a dm) dms'
+    end.
+
+  Fixpoint inlineDmsRep {retT} (a: Action type retT) (dms: list (DefMethT type))
            (countdown: nat): Action type retT :=
     match countdown with
       | O => a
-      | S cd => inlineAction (inlineActionOnce a dms) dms cd
+      | S cd => inlineDmsRep (inlineDms a dms) dms cd
     end.
 
-  Definition inlineRule (r: Attribute (Action type (Bit 0)))
-             (dms: list (DefMethT type)): Attribute (Action type (Bit 0)) :=
-    match r with
-      | {| attrName := rn; attrType := ra |} =>
-        {| attrName := rn;
-           attrType := inlineAction ra dms (List.length dms) |}
-    end.
+  Section Countdown.
+    Variable countdown: nat.
 
-  Fixpoint inlineRules (rules: list (Attribute (Action type (Bit 0))))
-           (dms: list (DefMethT type)): list (Attribute (Action type (Bit 0))) :=
-    match rules with
-      | nil => nil
-      | r :: rules' => (inlineRule r dms) :: (inlineRules rules' dms)
-    end.
+    Definition inlineToRule (r: Attribute (Action type (Bit 0)))
+               (dms: list (DefMethT type)): Attribute (Action type (Bit 0)) :=
+      match r with
+        | {| attrName := rn; attrType := ra |} =>
+          {| attrName := rn;
+             attrType := inlineDmsRep ra dms countdown |}
+      end.
 
-  Lemma inlineRules_In:
-    forall r rules dms, In r rules -> In (inlineRule r dms) (inlineRules rules dms).
-  Proof.
-    induction rules; intros; inv H.
-    - left; reflexivity.
-    - right; apply IHrules; auto.
-  Qed.
+    Fixpoint inlineToRules (rules: list (Attribute (Action type (Bit 0))))
+             (dms: list (DefMethT type)): list (Attribute (Action type (Bit 0))) :=
+      match rules with
+        | nil => nil
+        | r :: rules' => (inlineToRule r dms) :: (inlineToRules rules' dms)
+      end.
 
-  Definition inlineMethod (n: string) {argT retT} (m: type argT -> Action type retT)
-             (dms: list (DefMethT type)): type argT -> Action type retT :=
-    fun a => inlineAction (m a) dms (List.length dms).
+    Lemma inlineToRules_In:
+      forall r rules dms, In r rules -> In (inlineToRule r dms) (inlineToRules rules dms).
+    Proof.
+      induction rules; intros; inv H.
+      - left; reflexivity.
+      - right; apply IHrules; auto.
+    Qed.
 
-  Fixpoint inlineDms (dms: list (DefMethT type)): list (DefMethT type) :=
-    match dms with
-      | nil => nil
-      | {| attrName := n; attrType := {| objType := s; objVal := a |} |} :: dms' =>
-        {| attrName := n; attrType := {| objType := s; objVal := inlineMethod n a dms |} |}
-          :: (inlineDms dms')
-    end.
+    Definition inlineToDm (n: string) {argT retT} (m: type argT -> Action type retT)
+               (dms: list (DefMethT type)): type argT -> Action type retT :=
+      fun a => inlineDmsRep (m a) dms countdown.
 
-  Definition inlineMod (m1 m2: Modules type): Modules type :=
-    match m1, m2 with
-      | Mod regs1 r1 dms1, Mod regs2 r2 dms2 =>
-        Mod (regs1 ++ regs2) (inlineRules (r1 ++ r2) (dms1 ++ dms2)) (inlineDms (dms1 ++ dms2))
-      | _, _ => m1 (* undefined *)
-    end.
+    Fixpoint inlineToDms (dms: list (DefMethT type)): list (DefMethT type) :=
+      match dms with
+        | nil => nil
+        | {| attrName := n; attrType := {| objType := s; objVal := a |} |} :: dms' =>
+          {| attrName := n; attrType := {| objType := s; objVal := inlineToDm n a dms |} |}
+            :: (inlineToDms dms')
+      end.
 
-  (* necessary condition *)
-  Fixpoint noCalls {retT} (a: Action type retT) :=
-    match a with
-      | MCall _ _ _ _ => false
-      | Let_ _ ar cont => noCalls (cont (getDefault _))
-      | ReadReg reg k cont => noCalls (cont (getDefault _))
-      | WriteReg reg _ e cont => noCalls cont
-      | IfElse ce _ ta fa cont => (noCalls ta) && (noCalls fa) && (noCalls (cont (getDefault _)))
-      | Assert_ ae cont => noCalls cont
-      | Return e => true
-    end.
+    Definition inlineMod (m1 m2: Modules type): Modules type :=
+      match m1, m2 with
+        | Mod regs1 r1 dms1, Mod regs2 r2 dms2 =>
+          Mod (regs1 ++ regs2) (inlineToRules (r1 ++ r2) (dms1 ++ dms2))
+              (inlineToDms (dms1 ++ dms2))
+        | _, _ => m1 (* undefined *)
+      end.
 
-  Fixpoint noCallsRules (rules: list (Attribute (Action type (Bit 0)))) :=
-    match rules with
-      | nil => true
-      | {| attrType := r |} :: rules' => (noCalls r) && (noCallsRules rules')
-    end.
-
-  Fixpoint noCallsDms (dms: list (DefMethT type)) :=
-    match dms with
-      | nil => true
-      | {| attrType := {| objVal := dm |} |} :: dms' =>
-        (noCalls (dm (getDefault _))) && (noCallsDms dms')
-    end.
-
-  Fixpoint noCallsMod (m: Modules type) :=
-    match m with
-      | Mod _ rules dms => (noCallsRules rules) && (noCallsDms dms)
-      | ConcatMod m1 m2 => (noCallsMod m1) && (noCallsMod m2)
-    end.
+  End Countdown.
 
 End Phoas.
 
+Section PhoasTT.
+
+  Definition typeTT (k: Kind): Type :=
+    match k with
+      | _ => unit
+    end.
+
+  (* Well-formedness w.r.t. method calls *)
+  Section Wfm.
+    Fixpoint nodupString (l: list string): bool :=
+      match l with
+        | nil => true
+        | hd :: tl => if in_dec string_dec hd tl then false else nodupString tl
+      end.
+
+    Fixpoint collectCalls (calls: list (list string)) {retT} (a: Action typeTT retT)
+    : list (list string) :=
+      match a with
+        | MCall name _ _ cont =>
+          collectCalls (map (fun l => name :: l) calls) (cont tt)
+        | Let_ _ ar cont => collectCalls calls (cont tt)
+        | ReadReg reg k cont => collectCalls calls (cont tt)
+        | WriteReg reg _ e cont => collectCalls calls cont
+        | IfElse ce _ ta fa cont =>
+          app (collectCalls (collectCalls calls ta) (cont tt))
+              (collectCalls (collectCalls calls fa) (cont tt))
+        | Assert_ _ cont => collectCalls calls cont
+        | Return _ => calls
+      end.
+
+    Definition wfmAction {retT} (a: Action typeTT retT) :=
+      forallb (fun l => nodupString l) (collectCalls ((@nil string) :: nil) a).
+
+    Inductive WfmAction: list string -> forall {retT}, Action typeTT retT -> Prop :=
+    | WfmMCall:
+        forall ll name sig ar {retT} cont t (Hnin: ~ In name ll),
+          WfmAction (name :: ll) (cont t) ->
+          WfmAction ll (MCall (lretT:= retT) name sig ar cont)
+    | WfmLet:
+        forall ll {argT retT} ar cont t,
+          WfmAction ll (cont t) ->
+          WfmAction ll (Let_ (lretT':= argT) (lretT:= retT) ar cont)
+    | WfmReadReg:
+        forall ll {retT} reg k cont t,
+          WfmAction ll (cont t) ->
+          WfmAction ll (ReadReg (lretT:= retT) reg k cont)
+    | WfmWriteReg:
+        forall ll {writeT retT} reg e cont,
+          WfmAction ll cont ->
+          WfmAction ll (WriteReg (k:= writeT) (lretT:= retT) reg e cont)
+    | WfmIfElse:
+        forall ll {retT1 retT2} ce ta fa cont,
+          WfmAction ll (appendAction (retT1:= retT1) (retT2:= retT2) ta cont) ->
+          WfmAction ll (appendAction (retT1:= retT1) (retT2:= retT2) fa cont) ->
+          WfmAction ll (IfElse ce ta fa cont)
+    | WfmAssert:
+        forall ll {retT} e cont,
+          WfmAction ll cont ->
+          WfmAction ll (Assert_ (lretT:= retT) e cont)
+    | WfmReturn:
+        forall ll {retT} (e: Expr typeTT retT), WfmAction ll (Return e).
+
+    Lemma wfmAction_WfmAction:
+      forall {retT} (a: Action typeTT retT), wfmAction a = true -> WfmAction nil a.
+    Proof.
+      admit.
+    Qed.
+
+  End Wfm.
+
+  Section NoCalls.
+    (* Necessary condition for inlining correctness *)
+    Fixpoint noCalls {retT} (a: Action typeTT retT) :=
+      match a with
+        | MCall _ _ _ _ => false
+        | Let_ _ ar cont => noCalls (cont tt)
+        | ReadReg reg k cont => noCalls (cont tt)
+        | WriteReg reg _ e cont => noCalls cont
+        | IfElse ce _ ta fa cont => (noCalls ta) && (noCalls fa) && (noCalls (cont tt))
+        | Assert_ ae cont => noCalls cont
+        | Return e => true
+      end.
+
+    Fixpoint noCallsRules (rules: list (Attribute (Action typeTT (Bit 0)))) :=
+      match rules with
+        | nil => true
+        | {| attrType := r |} :: rules' => (noCalls r) && (noCallsRules rules')
+      end.
+
+    Fixpoint noCallsDms (dms: list (DefMethT typeTT)) :=
+      match dms with
+        | nil => true
+        | {| attrType := {| objVal := dm |} |} :: dms' =>
+          (noCalls (dm tt)) && (noCallsDms dms')
+      end.
+
+    Fixpoint noCallsMod (m: Modules typeTT) :=
+      match m with
+        | Mod _ rules dms => (noCallsRules rules) && (noCallsDms dms)
+        | ConcatMod m1 m2 => (noCallsMod m1) && (noCallsMod m2)
+      end.
+
+  End NoCalls.
+
+End PhoasTT.
+
 Require Import Semantics.
+
+Inductive WfmActionSem: list string -> forall {retT}, Action type retT -> list string -> Prop :=
+| WfmMCallSem:
+    forall ll rl name sig ar {retT} cont (Hnin: ~ In name ll),
+      (forall t, WfmActionSem (name :: ll) (cont t) rl) ->
+      WfmActionSem ll (MCall (lretT:= retT) name sig ar cont) rl
+| WfmLetSem:
+    forall ll rl {argT retT} ar cont,
+      (forall t, WfmActionSem ll (cont t) rl) ->
+      WfmActionSem ll (Let_ (lretT':= argT) (lretT:= retT) ar cont) rl
+| WfmReadRegSem:
+    forall ll rl {retT} reg k cont,
+      (forall t, WfmActionSem ll (cont t) rl) ->
+      WfmActionSem ll (ReadReg (lretT:= retT) reg k cont) rl
+| WfmWriteRegSem:
+    forall ll rl {writeT retT} reg e cont,
+      WfmActionSem ll cont rl ->
+      WfmActionSem ll (WriteReg (k:= writeT) (lretT:= retT) reg e cont) rl
+| WfmIfElseSem:
+    forall ll trl frl rl {retT1 retT2} ce ta fa cont,
+      WfmActionSem (retT:= retT1) ll ta trl ->
+      WfmActionSem (retT:= retT1) ll fa frl ->
+      (forall t, WfmActionSem (retT:= retT2) (trl ++ frl) (cont t) rl) ->
+      (* WfmActionSem ll (appendAction (retT1:= retT1) (retT2:= retT2) ta cont) -> *)
+      (* WfmActionSem ll (appendAction (retT1:= retT1) (retT2:= retT2) fa cont) -> *)
+      WfmActionSem ll (IfElse ce ta fa cont) rl
+| WfmAssertSem:
+    forall ll rl {retT} e cont,
+      WfmActionSem ll cont rl ->
+      WfmActionSem ll (Assert_ (lretT:= retT) e cont) rl
+| WfmReturnSem:
+    forall ll rl {retT} (e: Expr type retT), ll = rl -> WfmActionSem ll (Return e) rl.
+
+Definition WfmActionSem' {retT} (a: Action type retT) := exists rl, WfmActionSem nil a rl.
+
+Lemma WfmActionSem_init:
+  forall {retK} (a: Action type retK) ll rl
+         (Hwfm: WfmActionSem ll a rl),
+    WfmActionSem' a.
+Proof.
+  admit.
+Qed.
+
+Lemma WfmActionSem_MCall:
+  forall {retK} olds a news calls (retV: type retK) dmn rl
+         (Hsem: SemAction olds a news calls retV)
+         (Hwfm: WfmActionSem [dmn] a rl),
+    complement calls [dmn] = calls.
+Proof.
+  induction a; intros; invertAction Hsem; inv Hwfm; destruct_existT.
+
+  - admit.
+  - eapply H; eauto.
+  - eapply H; eauto.
+  - eapply IHa; eauto.
+  - admit.
+  - eapply IHa; eauto.
+  - map_simpl_G; reflexivity.
+Qed.
 
 Section Preliminaries.
 
   Lemma action_olds_ext:
-    forall retK olds1 olds2 a news calls (retV: type retK),
+    forall retK a olds1 olds2 news calls (retV: type retK),
       FnMap.Sub olds1 olds2 ->
       SemAction olds1 a news calls retV ->
       SemAction olds2 a news calls retV.
   Proof.
-    admit.
+    induction a; intros.
+    - invertAction H1; econstructor; eauto.
+    - invertAction H1; econstructor; eauto.
+    - invertAction H1; econstructor; eauto.
+      repeat autounfold with MapDefs; repeat autounfold with MapDefs in H1.
+      rewrite <-H1; symmetry; apply H0; unfold InMap, find; rewrite H1; discriminate.
+    - invertAction H0; econstructor; eauto.
+    - invertAction H1.
+      remember (evalExpr e) as cv; destruct cv; dest.
+      + eapply SemIfElseTrue; eauto.
+      + eapply SemIfElseFalse; eauto.
+    - invertAction H0; econstructor; eauto.
+    - invertAction H0; econstructor; eauto.
   Qed.
 
   Lemma appendAction_prop:
@@ -195,6 +357,216 @@ Section Preliminaries.
       
   Qed.
 
+  Lemma SemMod_singleton:
+    forall rules olds news dm dmMap cmMap,
+      SemMod rules olds None news (dm :: nil) dmMap cmMap ->
+      DomainOf dmMap ((attrName dm) :: nil) ->
+      exists argV retV,
+        dm = {| attrName := attrName dm;
+                attrType := {| objType := {| arg := arg (objType (attrType dm));
+                                             ret := ret (objType (attrType dm)) |};
+                               objVal := objVal (attrType dm) |} |} /\
+        dmMap = add (attrName dm) {| objVal := (argV, retV) |} empty /\
+        SemAction olds (objVal (attrType dm) argV) news cmMap retV.
+  Proof.
+    intros.
+    invertSemMod H.
+
+    - invertSemMod HSemMod.
+      exists argV; exists retV.
+      split.
+      
+      + destruct dm as [dmn [[ ] ]]; simpl; reflexivity.
+      + split; [reflexivity|].
+        map_simpl_G; assumption.
+
+    - invertSemMod HSemMod; exfalso.
+      specialize (H0 (attrName dm)); destruct H0.
+      specialize (H0 (or_introl eq_refl)).
+      unfold InMap in H0; elim H0; reflexivity.
+  Qed.
+
+  Lemma inlineDm_prop:
+    forall olds1 olds2 retK2 a2
+           dm rules news1 news2 dmMap1 cmMap1 cmMap2
+           (retV2: type retK2),
+      Disj olds1 olds2 -> Disj news1 news2 -> Disj cmMap1 cmMap2 ->
+      
+      WfmActionSem' a2 ->
+      SemAction olds2 a2 news2 cmMap2 retV2 ->
+      
+      find (attrName dm) cmMap2 = find (attrName dm) dmMap1 -> (* labels match *)
+      DomainOf dmMap1 ((attrName dm) :: nil) -> (* dm is actually called *)
+      
+      SemMod rules olds1 None news1 (dm :: nil) dmMap1 cmMap1 ->
+      SemAction (union olds1 olds2) (inlineDm a2 dm)
+                (union news1 news2)
+                (union cmMap1 (complement cmMap2 ((attrName dm) :: nil)))
+                retV2.
+  Proof.
+    intros; pose proof (SemMod_singleton H6 H5); clear H5 H6; dest.
+    destruct dm as [dmn [[ ]]]; simpl in *; inv H5.
+    map_simpl H4.
+
+    generalize dependent olds2; generalize dependent news2; generalize dependent cmMap2.
+    induction a2; intros.
+
+    - invertAction H5.
+      simpl; destruct (string_dec meth dmn); [subst|].
+
+      + clear H. (* don't need IH for this case *)
+
+        map_simpl H4.
+        apply opt_some_eq in H4; subst.
+        apply typed_type_eq in H4; dest.
+        generalize dependent H5; subst; intros.
+        inv H.
+
+        destruct (SignatureT_dec _ _); [|elim n; reflexivity].
+        simpl in *; rewrite <-Eqdep.EqdepTheory.eq_rect_eq; clear e0.
+
+        econstructor; eauto.
+        apply appendAction_prop with (retV1:= x0); auto.
+        map_simpl_G.
+
+        inv H2; inv H; destruct_existT.
+        specialize (H12 x0).
+        pose proof (WfmActionSem_MCall H5 H12); rewrite H.
+        assumption.
+
+      + rewrite find_add_2 in H4
+          by (unfold string_eq; destruct (string_dec _ _); [elim n; assumption|reflexivity]).
+        econstructor; eauto.
+
+        * instantiate (1:= union cmMap1 (complement x2 [dmn])); instantiate (1:= x1).
+
+          clear -n H1.
+          unfold Disj in H1.
+          apply Equal_eq; repeat autounfold with MapDefs; intros.
+          specialize (H1 k).
+          destruct H1.
+
+          { unfold find in H; rewrite H.
+            destruct (in_dec _ _ _).
+            { inv i; [|inv H0].
+              unfold string_eq; destruct (string_dec _ _); [elim n; assumption|reflexivity].
+            }
+            { unfold string_eq; destruct (string_dec _ _); reflexivity. }
+          }
+          { destruct (cmMap1 k).
+            { unfold string_eq; destruct (string_dec _ _); [|reflexivity].
+              subst; map_simpl H; discriminate.
+            }
+            { destruct (in_dec _ _ _).
+              { inv i; [|inv H0].
+                unfold string_eq; destruct (string_dec _ _); [elim n; assumption|reflexivity].
+              }
+              { unfold string_eq; destruct (string_dec _ _); reflexivity. }
+            }
+          }
+
+        * apply H; auto.
+          { inv H2; inv H6; destruct_existT.
+            specialize (H14 x1).
+            eapply WfmActionSem_init; eauto.
+          }
+          { eapply Disj_add_2; eauto. }
+
+    - invertAction H5; inv H2; inv H6; destruct_existT.
+      simpl. econstructor; eauto.
+      eapply H; eauto.
+      eexists; apply H13.
+
+    - invertAction H5; inv H2; inv H8; destruct_existT.
+      simpl; econstructor; eauto.
+      + apply Disj_find_union; eauto.
+      + eapply H; eauto.
+        eexists; apply H14.
+
+    - invertAction H3; inv H2; inv H5; destruct_existT.
+      simpl; econstructor; eauto.
+
+      + instantiate (1:= union news1 x1).
+        apply Equal_eq; repeat autounfold with MapDefs; intros.
+        specialize (H0 k0); destruct H0.
+        * unfold find in H0; rewrite H0.
+          unfold string_eq; destruct (string_dec _ _); reflexivity.
+        * destruct (news1 k0).
+          { unfold string_eq; destruct (string_dec _ _); [|reflexivity].
+            subst; map_simpl H0; inv H0.
+          }
+          { unfold string_eq; destruct (string_dec _ _); reflexivity. }
+      + apply IHa2; auto.
+        * eexists; apply H13.
+        * eapply Disj_add_2; eauto.
+
+    - invertAction H5; inv H2; inv H6; destruct_existT.
+      remember (evalExpr e) as cv; destruct cv; dest; subst.
+
+      + simpl; eapply SemIfElseTrue.
+
+        * auto.
+        * eapply IHa2_1.
+          { eexists; exact H15. }
+          { instantiate (1:= x2); eapply Disj_union_1; eauto. }
+          { admit. (* double-call problem *) }
+          { instantiate (1:= x1); eapply Disj_union_1; eauto. }
+          { assumption. }
+          { exact H2. }
+        * eapply H.
+          { eapply WfmActionSem_init; eauto. }
+          { instantiate (1:= x4); eapply Disj_union_2; eauto. }
+          { admit. (* double-call problem *) }
+          { instantiate (1:= x3); eapply Disj_union_2; eauto. }
+          { assumption. }
+          { exact H5. }
+        * admit. (* double-state problem *)
+        * admit. (* double-call problem *)
+
+      + simpl; eapply SemIfElseFalse.
+
+        * auto.
+        * eapply IHa2_2.
+          { eexists; exact H16. }
+          { instantiate (1:= x2); eapply Disj_union_1; eauto. }
+          { admit. (* double-call problem *) }
+          { instantiate (1:= x1); eapply Disj_union_1; eauto. }
+          { assumption. }
+          { exact H2. }
+        * eapply H.
+          { eapply WfmActionSem_init; eauto. }
+          { instantiate (1:= x4); eapply Disj_union_2; eauto. }
+          { admit. (* double-call problem *) }
+          { instantiate (1:= x3); eapply Disj_union_2; eauto. }
+          { assumption. }
+          { exact H5. }
+        * admit. (* double-state problem *)
+        * admit. (* double-call problem *)
+
+    - invertAction H3; inv H2; inv H6; destruct_existT.
+      simpl; econstructor; eauto.
+      eapply IHa2; eauto; eexists; exact H12.
+
+    - invertAction H3; simpl; map_simpl_G.
+      map_simpl H4; inv H4.
+
+  Qed.
+  
+  Lemma inlineDms_prop:
+    forall dms olds1 olds2 retK2 a2 rules news1 news2 dmMap1 cmMap1 cmMap2
+           (retV2: type retK2),
+      SemAction olds2 a2 news2 cmMap2 retV2 ->
+      dmMap1 = restrict cmMap2 (map (@attrName _) dms) ->
+      SemMod rules olds1 None news1 dms dmMap1 cmMap1 ->
+      SemAction (union olds1 olds2) (inlineDms a2 dms)
+                (union news1 news2) (union cmMap1 (complement cmMap2 (map (@attrName _) dms)))
+                retV2.
+  Proof.
+    admit.
+  Qed.
+
+  (* TODO: extend *)
+
 End Preliminaries.
 
 Section Facts.
@@ -202,13 +574,13 @@ Section Facts.
             (r1 r2: list (Attribute (Action type (Bit 0))))
             (dms1 dms2: list (DefMethT type)).
 
-  Definition getDefault := (fun k: Kind => evalConstT (getDefaultConst k)).
+  Variable countdown: nat. (* TODO: weird *)
 
   Definition m1 := Mod regs1 r1 dms1.
   Definition m2 := Mod regs2 r2 dms2.
 
   Definition cm := ConcatMod m1 m2.
-  Definition im := @inlineMod type m1 m2.
+  Definition im := @inlineMod type countdown m1 m2.
 
   Lemma inline_correct_rule:
     forall r or nr cmMap,
@@ -230,7 +602,7 @@ Section Facts.
         eapply SemAddRule.
         * assert (Hin: In (s :: ruleBody)%struct (r1 ++ r2)) by
               (apply in_or_app; right; assumption); clear HInRule.
-          pose proof (inlineRules_In _ _ (dms1 ++ dms2) Hin).
+          pose proof (inlineToRules_In countdown _ _ (dms1 ++ dms2) Hin).
           exact H0.
         * instantiate (3:= disjUnion news1 (union news news0)
                                      (map (attrName (Kind:=Typed ConstT)) (getRegInits m1))).
@@ -241,16 +613,6 @@ Section Facts.
                              (listSub (getCmsR r1 ++ getCmsM dms1)
                                       (map (@attrName _) dms2))).
           instantiate (1:= retV).
-
-          
-
-          unfold FiltDm in Hfd; simpl in Hfd.
-          clear Hfc.
-          
-
-          
-
-            
           admit.
         * instantiate (2:= empty); instantiate (1:= empty).
           apply SemMod_empty.
